Add attestation steps to state transition model

src/AttarchProperties.v
@@ -9,117 +9,77 @@ Open Scope string_scope.
 Open Scope tprop_scope.
 Open Scope env_scope.
 
-Definition useram_key_secure : tprop attarch_state := <[λ '(_, Γ),
-  forall c,
-    read Γ c "useram_key" good_useram_key -> 
-    c = "useram"
-]>.
+
+Ltac star_notation := 
+  repeat change (clos_refl_trans_n1 _ ?R) with (R^*) in *.
+
 
 Definition diverged : tprop attarch_state :=
   <[λ '(l, _), l = attarch_bot]>.
 
-Ltac star_notation := 
-  repeat change (clos_refl_trans_n1 _ ?R) with (R^*) in *.
-  
-Theorem useram_key_never_compromised:
-  attarch_trans @attarch_good_init_state ⊨ AG useram_key_secure.
+
+Definition platam_key_secure : tprop attarch_state := <[λ '(_, Γ),
+  forall c key_t (key: key_t),
+    read Γ c "platam_key" key -> 
+    c = "platam"
+]>.
+
+Theorem platam_key_uncompromised: forall s0,
+  is_init_attarch_state s0 ->
+  attarch_trans @s0 ⊨ AG platam_key_secure.
 Proof.
-  tcut (AG <[λ '(_, Γ), forall acc b, Γ "useram_key" = Some (acc, b) ->
-             acc = private "useram"]>).
-  { apply AG_weaken.
-    intros [l Γ].
-    tintro H.
-    tentails! in *.
-    intros * (acc & Hlookup & Hacc).
-    do 2 especialize H; forward H by eassumption.
-    subst.
-    unfold private in Hacc.
-    follows apply refl_string_eq in Hacc. }
+  intros s0 s0_init.
   apply star__AG.
-  intros * Hstar.
+  intros s Hstar.
   induct! Hstar; star_notation.
-  - follows tentails!.
-  - invc H.
-    + follows tentails!.
-    + follows tentails!.
-    + invc H;
-      tentails! in *;
-      intros;
-      eapply IHHstar;
-      follows write_unchanged_facts.
-    + invc H.
-      invc H0.
+  - destruct or s0_init;
+    rewritec s0_init;
+    follows tentails!.
+  - invc H; try rw_solver.
+    + invc H; try rw_solver.
       tentails! in *.
-      intros.
-      destruct H5 as (acc' & curr & Hlookup & Hacc & ->).
-      tedious.
-    + follows tentails! in *.
+      intros .
+      destruct H5 as (acc & a & lookup & Hacc & ->).
+      destruct a as [? a]; change ⟨_, a⟩ with (box a) in *.
+      simpl_rws.
+      follows eapply IHHstar.
+    + invc H; invc H0; rw_solver.
 Qed.
-      
-(* Theorem useram_key_never_compromised':
-  attarch_trans @attarch_init_state ⊨ A[useram_key_secure W diverged].
+
+
+Definition useram_key_secure : tprop attarch_state := <[λ '(_, Γ),
+  forall c key_t (key: key_t),
+    read Γ c "useram_key" key -> 
+    c = "useram"
+]>.
+
+(* Definition finish_setup : tprop attarch_state := <[λ '(l, _),
+  exists l', l = sel4_run l' (vm_run useram_listen)
+]>. *)
+
+Definition setup_finished : tprop attarch_state := <[λ '(l, _),
+  exists pl ul, 
+    l = sel4_run pl (vm_run ul) /\
+    ul <> useram_wait_key
+]>.
+
+Theorem useram_key_uncompromised_setup : forall s0,
+  is_init_attarch_state s0 ->
+  attarch_trans @s0 ⊨ A[useram_key_secure W setup_finished].
 Proof.
-  apply AW_intro; split.
-  - left. follows tentails!.
-  - intros s' seq IH s'' step.
-    invc step.
-    + left.
-      tentails!.
-      intros * [=] H'; subst!.
-      follows econtradiction no_lookup_no_read.
-    + left.
-      tentails!.
-      intros * [=] H'; subst!.
-      follows econtradiction no_lookup_no_read.
-    + left.
-      invc H.
-      * especialize IH; forward IH by apply in_seq_head.
-        destruct IH as [IH _].
-        tentails! in *.
-        intros * [=] H'; subst!.
-        eapply IH; [reflexivity|].
-        follows eapply write_unchanged_read'.
-      * especialize IH; forward IH by apply in_seq_head.
-        destruct IH as [IH _].
-        tentails! in *.
-        intros * [=] H'; subst!.
-        follows eapply IH.
-    + left.
-      invc H.
-      invc H0.
-      especialize IH; forward IH by apply in_seq_head.
-      destruct IH as [IH _].
-      tentails! in *.
-      intros * [=] H'; subst!.
-      follows eapply IH.
-    + right.
-      follows tentails!.
-Qed. *)
-
-(* Theorems:
-   1. platam key always secure 
-   2. useram key perfectly secure until release 
-     - This may be trivial since useram doesn't have key until release
-     - Maybe not, if the theorem talks about the internal representation 
-       stored by the useram
-   3. Useram key leak is observed unless malicious component acts, steals, 
-      and repairs before platAM notices
-   4. useram evidence is trustworthy unless malicious actor interferes 
-      and useram interacts before the platform am checks in
- *)
-
-(* Definition platam_key_secure : tprop attarch_state := <[λ '(l, _),
-    forall Γ l' s c,
-      l = sel4_run (l', Γ) s ->
-      read Γ c "useram_key" good_useram_key -> 
-      c = "useram"
-  ]>. *)
-
-
-(* Doesn't separation of gammas make this difficult to talk about *every* environment?
-   Joining of gammas isn't necessarily at odds with composition. Just need to redefine.
-*)
-
+  intros s0 s0_init.
+  apply AW_intro_weak.
+  - left.
+    destruct or s0_init; rewritec s0_init;
+    follows tentails!.
+  - intros * Hstar [Hsecure Hnot_finished] * H.
+    invc H; try (left; rw_solver).
+    + left. invc H; rw_solver. 
+    + invc H; invc H0; try (left + right; rw_solver).
+      (* not true at the moment. Need platam to inspect useram
+         before releasing key!
+       *)
+Abort.
 
 Close Scope tprop_scope.
 Close Scope string_scope.
