src/AttarchTrans.v
@@ -29,6 +29,8 @@ Inductive useram_key_decr_key_t :=
   | good_decr_key
   | encr_decr_key
   | bad_decr_key.
+Inductive attest_req_t :=
+  | attest_req.
 
 
 (* Transition definitions *)
@@ -36,10 +38,11 @@ Inductive useram_key_decr_key_t :=
 Inductive platam_label :=
   | platam_init 
   | platam_meas_release
-  | platam_listen.
+  | platam_listen
+  | platam_deep_attest.
 
 Definition platam_init_env : env :=
-  private "platam" ? (
+  only "platam" ? (
     "platam_key" ↦ encr_platam_key ;;
     "useram_key_decr_key" ↦ encr_decr_key
   ).
@@ -71,22 +74,36 @@ Inductive platam_trans : relation (platam_label × env) :=
       write Γ "platam" "vmm_dataport" (decrypt_useram_key_decr_key decr_key platam_key) Γ' ->
       platam_trans 
         (platam_meas_release, Γ)
+        (platam_listen, Γ')
+  | platam_get_deep_attest_req : forall Γ,
+      read Γ "platam" "vmm_dataport" attest_req ->
+      platam_trans
+        (platam_listen, Γ)
+        (platam_deep_attest, Γ)
+  | platam_do_deep_attest : forall Γ Γ' (meas: bool),
+      read  Γ "platam" "good_os" meas ->
+      write Γ "platam" "vmm_dataport" meas Γ' ->
+      platam_trans
+        (platam_deep_attest, Γ)
         (platam_listen, Γ').
-
-(* TODO, bad_platam_trans, *)
 
 Inductive useram_label := 
   | useram_wait_key
-  | useram_listen.
+  | useram_listen
+  | useram_shallow_attest
+  | useram_deep_attest.
 
 Definition useram_init_env : env := 
-  private "useram" ? "useram_key" ↦ encr_useram_key.
+  only "useram" ? "useram_key" ↦ encr_useram_key.
 
 Definition decrypt_useram_key key decr_key : useram_key_t := 
   match (key, decr_key) with 
   | (encr_useram_key, good_decr_key) => good_useram_key
   | _ => bad_useram_key
   end.
+
+Definition shallow_attest (good_os good_target good_meas: bool) :=
+  good_os -> good_target -> good_meas.
 
 Inductive useram_trans : relation (useram_label × env) :=
   | useram_get_key : forall Γ Γ' encr_key decr_key,
@@ -95,7 +112,43 @@ Inductive useram_trans : relation (useram_label × env) :=
       write Γ "useram" "useram_key" (decrypt_useram_key encr_key decr_key) Γ' ->
       useram_trans 
         (useram_wait_key, Γ)
-        (useram_listen, Γ').
+        (useram_listen, Γ')
+  | useram_get_shallow_req : forall Γ,
+      useram_trans
+        (useram_listen, Γ)
+        (useram_shallow_attest, Γ)
+  | useram_do_shallow_attest : forall Γ Γ' os target meas,
+      read  Γ "useram" "good_os" os ->
+      read  Γ "useram" "good_os" target ->
+      shallow_attest os target meas ->
+      write Γ "useram" "shallow_attest_result" meas Γ' ->
+      useram_trans
+        (useram_shallow_attest, Γ)
+        (useram_listen, Γ)
+  | useram_get_deep_req : forall Γ Γ',
+      write Γ "useram" "vmm_dataport" attest_req Γ' ->
+      useram_trans
+        (useram_listen, Γ)
+        (useram_deep_attest, Γ')
+  | useram_wait_deep_attest : forall Γ (meas: bool),
+      read Γ "useram" "vmm_dataport" meas ->
+      useram_trans
+        (useram_deep_attest, Γ)
+        (useram_listen, Γ).
+
+
+Inductive malicious_proc_trans : relation env :=
+  | corrupt_os : forall Γ Γ',
+      write Γ "malicious_proc" "good_os" false Γ' ->
+      malicious_proc_trans Γ Γ'
+  | leak_key : forall Γ Γ',
+      changeAcc Γ "useram_key" (λ acc, canRead "malicious_proc" ⊔ acc) Γ' ->
+      malicious_proc_trans Γ Γ'.
+
+
+Definition vm_init_env : env := 
+  readable ⊔ canWrite "malicious_proc" ? "good_os" ↦ true;;
+  useram_init_env.
 
 Inductive vm_label := 
   | vm_run : useram_label -> vm_label.
@@ -103,7 +156,11 @@ Inductive vm_label :=
 Inductive vm_trans : relation (vm_label × env) := 
   | useram_step : forall x y Γ Γ',
       useram_trans (x, Γ) (y, Γ') ->
-      vm_trans (vm_run x, Γ) (vm_run y, Γ').
+      vm_trans (vm_run x, Γ) (vm_run y, Γ')
+  | malicious_proc_step : forall x Γ Γ',
+      malicious_proc_trans Γ Γ' ->
+      vm_trans (vm_run x, Γ) (vm_run x, Γ').
+
 
 Inductive attarch_label :=
   | boot
@@ -118,20 +175,16 @@ Inductive attarch_trans : relation attarch_state :=
       attarch_trans
         (boot, Γ)
         (sel4_run platam_init (vm_run useram_wait_key),
-          allReadOnly ? "boot_token" ↦ good_boot_token ;;
-          platam_init_env ;;
-          useram_init_env ;;
-          Γ
+          readable ? "boot_token" ↦ good_boot_token;;
+          platam_init_env;; vm_init_env;; Γ
         )
   | boot_bad : forall Γ,
       read Γ "root_of_trust" "good_image" false -> 
       attarch_trans
         (boot, Γ)
         (sel4_run platam_init (vm_run useram_wait_key),
-          allReadOnly ? "boot_token" ↦ bad_boot_token ;;
-          platam_init_env ;;
-          useram_init_env ;;
-          Γ
+          readable ? "boot_token" ↦ bad_boot_token;;
+          platam_init_env;; vm_init_env;; Γ
         )
   | platam_step : forall x l l' Γ Γ',
       platam_trans (l, Γ) (l', Γ') ->
@@ -147,19 +200,20 @@ Inductive attarch_trans : relation attarch_state :=
       attarch_trans (l, Γ) (attarch_bot, Γ).
 
 Definition attarch_good_init_state : attarch_state := 
-  (boot, allReadOnly ? "good_image" ↦ true).
+  (boot, readable ? "good_image" ↦ true).
 
 Definition attarch_bad_init_state : attarch_state := 
-  (boot, allReadOnly ? "good_image" ↦ false).
+  (boot, readable ? "good_image" ↦ false).
+
+Definition is_init_attarch_state (s: attarch_state) : Prop := 
+  s = attarch_good_init_state \/ 
+  s = attarch_bad_init_state.
+
 
 Lemma attarch_trans_serial : 
   serial_witness attarch_trans.
 Proof using.
   follows cbv.
-  (* unfold serial_witness.
-  intros [l ?].
-  eexists.
-  apply attarch_diverge. *)
 Defined.
 
 Instance transition__attarch_trans : transition attarch_trans :=
