src/Privilege.v
@@ -17,14 +17,195 @@ Definition comp := string.
 
 Definition access := comp -> privilege -> bool.
 
-Definition allAcc : access := λ _ _, true.
 
-Definition allReadOnly : access := λ _ p,
+Definition acc_union (a1 a2: access) : access := λ c p,
+  orb (a1 c p) (a2 c p).
+Notation "a1 ⊔ a2" := (acc_union a1 a2)
+  (at level 50, left associativity).
+
+Definition acc_inter (a1 a2: access) : access := λ c p,
+  andb (a1 c p) (a2 c p).
+Notation "a1 ⊓ a2" := (acc_inter a1 a2)
+  (at level 40, left associativity).
+
+Definition acc_le (a1 a2: access) : Prop := forall c p,
+  (* Bool.le (a1 c p) (a2 c p). *)
+  (a1 c p) -> (a2 c p).
+Notation "a1 ⊑ a2" := (acc_le a1 a2)
+  (at level 70).
+
+Definition acc_bot : access := λ _ _, false.
+
+Definition acc_top : access := λ _ _, true.
+
+
+Lemma acc_union_assoc : forall a1 a2 a3,
+  a1 ⊔ (a2 ⊔ a3) = a1 ⊔ a2 ⊔ a3.
+Proof using.
+  intros *.
+  extensionality c p.
+  apply Bool.orb_assoc.
+Qed.
+
+Lemma acc_union_comm : forall a1 a2,
+  a1 ⊔ a2 = a2 ⊔ a1.
+Proof using.
+  intros *.
+  extensionality c p.
+  apply Bool.orb_comm.
+Qed.
+
+Lemma acc_bot_union_l : forall a,
+  acc_bot ⊔ a = a.
+Proof using.
+  intros *.
+  extensionality c p.
+  follows cbn.
+Qed.
+
+Lemma acc_bot_union_r : forall a,
+  a ⊔ acc_bot = a.
+Proof using.
+  intros *.
+  rewrite acc_union_comm.
+  apply acc_bot_union_l.
+Qed.
+
+Lemma acc_top_union_l : forall a,
+  acc_top ⊔ a = acc_top.
+Proof using.
+  intros *.
+  extensionality c p.
+  follows cbn.
+Qed.
+
+Lemma acc_top_union_r : forall a,
+  a ⊔ acc_top = acc_top.
+Proof using.
+  intros *.
+  rewrite acc_union_comm.
+  apply acc_top_union_l.
+Qed.
+
+Lemma acc_inter_assoc : forall a1 a2 a3,
+  a1 ⊓ (a2 ⊓ a3) = a1 ⊓ a2 ⊓ a3.
+Proof using.
+  intros *.
+  extensionality c p.
+  apply Bool.andb_assoc.
+Qed.
+
+Lemma acc_inter_comm : forall a1 a2,
+  a1 ⊓ a2 = a2 ⊓ a1.
+Proof using.
+  intros *.
+  extensionality c p.
+  apply Bool.andb_comm.
+Qed.
+
+Lemma acc_bot_inter_l : forall a,
+  acc_bot ⊓ a = acc_bot.
+Proof using.
+  intros *.
+  extensionality c p.
+  follows cbn.
+Qed.
+
+Lemma acc_bot_inter_r : forall a,
+  a ⊓ acc_bot = acc_bot.
+Proof using.
+  intros *.
+  rewrite acc_inter_comm.
+  apply acc_bot_inter_l.
+Qed.
+
+Lemma acc_top_inter_l : forall a,
+  acc_top ⊓ a = a.
+Proof using.
+  intros *.
+  extensionality c p.
+  follows cbn.
+Qed.
+
+Lemma acc_top_inter_r : forall a,
+  a ⊓ acc_top = a.
+Proof using.
+  intros *.
+  rewrite acc_inter_comm.
+  apply acc_top_inter_l.
+Qed.
+
+Lemma acc_bot_le : forall a,
+  acc_bot ⊑ a.
+Proof using.
+  tedious.
+Qed.
+
+Lemma acc_le_top : forall a,
+  a ⊑ acc_top.
+Proof using.
+  unfold acc_le.
+  intros *.
+  follows destruct (a c p).
+Qed.
+
+Lemma acc_union_le_l : forall a1 a2,
+  a1 ⊑ a1 ⊔ a2.
+Proof using.
+  unfold acc_le, acc_union.
+  intros *.
+  follows destruct (a1 c p).
+Qed.
+
+Lemma acc_union_le_r : forall a1 a2,
+  a2 ⊑ a1 ⊔ a2.
+Proof using.
+  unfold acc_le, acc_union.
+  intros *.
+  follows destruct (a1 c p), (a2 c p).
+Qed.
+
+Lemma acc_inter_le_l : forall a1 a2,
+  a1 ⊓ a2 ⊑ a1.
+Proof using.
+  unfold acc_le, acc_inter.
+  intros *.
+  follows destruct (a1 c p), (a2 c p).
+Qed.
+
+Lemma acc_inter_le_r : forall a1 a2,
+  a1 ⊓ a2 ⊑ a2.
+Proof using.
+  unfold acc_le, acc_inter.
+  intros *.
+  follows destruct (a1 c p), (a2 c p).
+Qed.
+
+
+Definition readable : access := λ _ p,
   match p with 
   | p_read => true 
   | _    => false 
   end.
 
-Definition private (c: comp): access := λ c' _, c =? c'.
-  
+Definition canRead (c: comp) : access := λ c' p,
+  match p with 
+  | p_read => c =? c'
+  | _ => false
+  end.
+
+Definition writable : access := λ _ p,
+  match p with 
+  | p_write => true 
+  | _    => false 
+  end.
+
+Definition canWrite (c: comp) : access := λ c' p,
+  match p with 
+  | p_write => c =? c'
+  | _ => false
+  end.
+
+Definition only (c: comp) : access := λ c' _, c =? c'.
+ 
 Close Scope string_scope.
